% Ctrl + alt + b to build & preview (Linux)
\documentclass[11pt,a4paper]{article}

\usepackage[margin=1in, paperwidth=8.3in, paperheight=11.7in]{geometry}
\usepackage{amsfonts}
\usepackage{amsmath}
\usepackage{fancyhdr}
\usepackage{enumitem}

\begin{document}

\pagestyle{fancy}
\setlength\parindent{0pt}
\allowdisplaybreaks

\renewcommand{\headrulewidth}{0pt}
\newcommand{\vect}[1]{\boldsymbol{#1}}
\newcommand{\subtitle}[2]{\textbf{#1}\textit{#2} \\}
\newcommand{\dotprod}[0]{\boldsymbol{\cdot}}

% Cover page title
\title{General - Notes}
\author{Dom Hutchinson}
\date{\today}
\maketitle

% Header
\fancyhead[L]{Dom Hutchinson}
\fancyhead[C]{General - Notes}
\fancyhead[R]{\today}

\section{Hyperbolic Trig}
\begin{alignat*}{3}
  &sinh(x) &&= \frac{e^{x} - e^{-x}}{2} \\
  &cosh(x) &&= \frac{e^{x} + e^{-x}}{2} \\
  &tanh(x) &&= \frac{sin(x)}{cosh(x)} &= \frac{e^{x} + e^{-x}}{e^{x} - e^{-x}} \\
  &cosech(x) &&= \frac{1}{sinh(x)} &= \frac{2}{e^{x} - e^{-x}} \\
  &sech(x) &&= \frac{1}{cosh(x)} &= \frac{2}{e^{x} + e^{-x}} \\
  &coth(x) &&= \frac{1}{tanh(x)} &= \frac{e^{x} - e^{-x}}{e^{x} + e^{-x}} \\
  &\frac{d}{dx}sinh(x) &&= cosh(x) \\
  &\frac{d}{dx}cosh(x) &&= sinh(x) \\
  &\frac{d}{dx}tanh(x) &&= sech^2(x) \\
  &\frac{d}{dx}cosech(x) &&= -cosech(x).coth^2(x) \\
  &\frac{d}{dx}sech(x) &&= -sech(x).tanh(x) \\
  &\frac{d}{dx}coth(x) &&= -cosech^2(x) \\
\end{alignat*}

\section{Trig Identities}
\begin{alignat*}{2}
  &sin(\alpha + \beta) &&= sin(\alpha)cos(\beta) + sin(\beta)cos(\alpha) \\
  &sin(\alpha - \beta) &&= sin(\alpha)cos(\beta) - sin(\beta)cos(\alpha) \\
  &cos(\alpha + \beta) &&= cos(\alpha)cos(\beta) - sin(\alpha)sin(\beta) \\
  &cos(\alpha - \beta) &&= cos(\alpha)cos(\beta) + sin(\alpha)sin(\beta) \\
  &sin^2(x) + cos^2(x) &&= 1 \\
  &tan^2(x) + 1 &&= sec^2(x) \\
  &1 + cot^2(x) &&= cosec^2(x) \\
  &sin(2x) &&= 2.sin(x).cos(x) \\
  &cos(2x) &&= cos^2(x) - sin^2(x)\\
  & &&= 2cos^2(x) - 1 \\
  & &&= 1 - 2sin^2(x) \\
  &sin^2(x) &&= \frac{1 - cos(2x)}{2} \\
  &cos^2(x) &&= \frac{1 + cos(2x)}{2} \\
  &tan^2(x) &&= \frac{1-cos(2x)}{1 + cos(2x)} \\
  &sin(x) + sin(y) &&= 2.sin\left(\frac{x+y}{2}\right).cos\left(\frac{x-y}{2}\right) \\
  &sin(x) - sin(y) &&= 2.sin\left(\frac{x-y}{2}\right).cos\left(\frac{x+y}{2}\right) \\
  &cos(x) + cos(y) &&= 2.cos\left(\frac{x+y}{2}\right).cos\left(\frac{x-y}{2}\right) \\
  &cos(x) - cos(y) &&= -2.sin\left(\frac{x+y}{2}\right).sin\left(\frac{x-y}{2}\right)
\end{alignat*}

\section{Limits}
\begin{alignat*}{2}
  &\lim_{x \to x_0} \frac{1-x}{1+x} &= 1 \\
  &\lim_{x \to \infty} \frac{1}{x} &= 0 \\
  &\lim_{x \to 0} \frac{sin(x)}{x} &= 1
\end{alignat*}

\section{Differentiation}
\subsection{Techniques}
Sum Rule
$$(f+g)' = f' + g'$$
%
Product Rule
$$(fg)' = f'g + fg'$$
%
Quotient Rule
$$\left(\frac{f}{g}\right)' = \frac{f'g - fg'}{g^2}$$
%
Chain Rule
$$\frac{d}{dx} f(g(x)) = f'(g(x)).g'(x)$$

\subsection{Common Results}
\begin{alignat*}{2}
  &\frac{d}{dx}(x^n) &&= nx^{n-1} \\
  &\frac{d}{dx}(e^x) &&= e^x \\
  &\frac{d}{dx}(ln(x)) &&= \frac{1}{x}\\
  &\frac{d}{dx}(sin(x)) &&= cos(x) \\
  &\frac{d}{dx}(cos(x)) &&= -sin(x) \\
  &\frac{d}{dx}(tan(x)) &&= sec^2(x) \\
  &\frac{d}{dx}(cot(x)) &&= -cosec^2(x) \\
  &\frac{d}{dx}(sec(x)) &&= tan(x).sec(x) \\
  &\frac{d}{dx}(cosec(x)) &&= -cosec(x).cot(x) \\
\end{alignat*}

\end{document}
